src/Concurrent/NodeSemantics.v
@@ -1,0 +1,170 @@
+From CoreErlang.Concurrent Require Export ProcessSemantics.
+
+Import ListNotations.
+
+Theorem Signal_eq_dec (s s' : Signal) : {s = s'} + {s <> s'}.
+Proof. decide equality; try apply Val_eq_dec; try apply Nat.eq_dec. decide equality. Qed.
+
+Definition update {T : Type} (pid : PID) (p : T) (n : PID -> T) : PID -> T :=
+  fun ι => if Nat.eqb pid ι then p else n ι.
+
+(** This representation assures that messages sent from the same process,
+    are delivered in the same order *)
+Definition Ether : Set := PID -> PID -> list Signal.
+Definition etherPop (source dest : PID) (n : Ether) :
+  option (Signal * Ether) :=
+match n source dest with
+| [] => None
+| x::xs => Some (x, update source (update dest xs (n source)) n)
+end.
+
+Definition ProcessPool : Set := (PID -> option Process).
+Definition Node : Set := Ether * ProcessPool.
+
+Definition nullpool : ProcessPool := fun ι => None.
+
+Notation "pid : p |||| n" := (update pid (Some p) n) (at level 32, right associativity).
+Notation "n -- pid" := (update pid None n) (at level 31, left associativity).
+Lemma update_same : forall T ι (p p' : T) Π, update ι p (update ι p' Π) = update ι p Π.
+Proof.
+  intros. unfold update. extensionality ι'.
+  break_match_goal; auto.
+Qed.
+Corollary par_same :  forall T ι (p p' : T) Π, ι : p |||| ι : p' |||| Π = ι : p |||| Π.
+Proof.
+  intros. apply update_same.
+Qed.
+
+Lemma update_swap : forall T ι ι' (p p' : T) Π, ι <> ι' ->
+   update ι p (update ι' p' Π) = update ι' p' (update ι p Π).
+Proof.
+  intros. unfold update. extensionality ι''.
+  break_match_goal; auto.
+  subst. break_match_goal; auto.
+  apply Nat.eqb_eq in Heqb0. apply Nat.eqb_eq in Heqb. congruence.
+Qed.
+Corollary par_swap :  forall ι ι' (p p' : (option Process)) Π, ι <> ι' ->
+   @update (option Process) ι p (update ι' p' Π) = update ι' p' (update ι p Π).
+Proof.
+  intros. now apply update_swap.
+Qed.
+Lemma nullpool_remove : forall ι, nullpool -- ι = nullpool.
+Proof.
+  intros. extensionality ι'.
+  unfold update. break_match_goal; auto.
+Qed.
+
+Definition etherAdd (source dest : PID) (m : Signal) (n : Ether) : Ether :=
+  update source (update dest (n source dest ++ [m]) (n source) ) n.
+
+Theorem update_noop :
+  forall T x (xval : T) n, n x = xval -> update x xval n = n.
+Proof.
+  intros. extensionality y.
+  unfold update. break_match_goal.
+  apply Nat.eqb_eq in Heqb. now subst.
+  reflexivity.
+Qed.
+
+Lemma etherPop_greater :
+  forall ι ether s ι' ether', etherPop ι ι' ether = Some (s, ether') ->
+  forall ι'' ι''' s', etherPop ι ι' (etherAdd ι'' ι''' s' ether) = Some (s, etherAdd ι'' ι''' s' ether').
+Proof.
+  intros. unfold etherPop, etherAdd, update in *.
+  destruct (Nat.eqb ι'' ι) eqn:Eq1; eqb_to_eq; subst.
+  * break_match_hyp; eqb_to_eq; subst; simpl. congruence.
+    inversion H.
+    break_match_goal.
+    - break_match_hyp.
+      destruct (ether ι ι'''); simpl in Heql0; inversion Heql0.
+      inversion Heql0.
+    - break_match_hyp; eqb_to_eq; subst.
+      + rewrite Heql in Heql0. simpl in Heql0. inversion Heql0.
+        do 3 f_equal.
+        extensionality ι0. break_match_goal; eqb_to_eq; subst; auto.
+        extensionality ι0'. break_match_goal; eqb_to_eq; subst; auto.
+        now do 2 rewrite Nat.eqb_refl.
+        rewrite Nat.eqb_refl. apply Nat.eqb_neq in Heqb. now rewrite Heqb.
+      + inversion Heql0.
+        do 3 f_equal.
+        extensionality ι0. break_match_goal; eqb_to_eq; subst; auto.
+        extensionality ι0'. break_match_goal; eqb_to_eq; subst; auto.
+        do 2 rewrite Nat.eqb_refl. apply Nat.eqb_neq in Heqb. now rewrite Heqb.
+        rewrite Nat.eqb_refl. apply not_eq_sym in Heqb.
+        apply Nat.eqb_neq in Heqb. rewrite Heqb.
+        apply Nat.eqb_neq in Heqb0. now rewrite Heqb0.
+  * break_match_hyp; eqb_to_eq; subst; simpl. congruence.
+    inversion H.
+    break_match_goal.
+    - do 3 f_equal.
+      extensionality ι0. break_match_goal; eqb_to_eq; subst; auto.
+      congruence. congruence.
+    - do 3 f_equal.
+      extensionality ι0. break_match_goal; eqb_to_eq; subst; auto.
+      extensionality ι0'. break_match_goal; eqb_to_eq; subst; auto.
+      apply not_eq_sym in Heqb.
+      apply Nat.eqb_neq in Heqb. rewrite Heqb. now rewrite Nat.eqb_refl.
+      apply not_eq_sym in Heqb.
+      apply Nat.eqb_neq in Heqb. rewrite Heqb.
+      apply Nat.eqb_neq in Heqb0. now rewrite Heqb0.
+Qed.
+
+Reserved Notation "n -[ a | ι ]ₙ-> n'" (at level 50).
+Inductive nodeSemantics : Node -> Action -> PID -> Node -> Prop :=
+(** sending any signal *)
+| n_send p p' ether prs (ι ι' : PID) t :
+  p -⌈ASend ι ι' t⌉-> p'
+->
+  (ether, ι : p |||| prs) -[ASend ι ι' t | ι]ₙ->  (etherAdd ι ι' t ether, ι : p' |||| prs)
+
+(** This leads to the loss of determinism: *)
+(** arrial of any signal *)
+| n_arrive ι ι0 p p' ether ether' prs t:
+  etherPop ι0 ι ether = Some (t, ether') ->
+  p -⌈AArrive ι0 ι t⌉-> p' ->
+  (ether, ι : p |||| prs) -[AArrive ι0 ι t | ι]ₙ-> (ether',
+                                            ι : p' |||| prs)
+
+(* TODO: link sent to non-existing process triggers exit, messages should be discarded when sent to non-existing process *)
+
+
+(** internal actions *)
+| n_other p p' a Π (ι : PID) ether:
+  p -⌈a⌉-> p' ->
+  (a = τ \/ a = ASelf ι \/ (exists t, a = AReceive t) \/ a = ATerminate \/ a = ASetFlag)
+->
+   (ether, ι : p |||| Π) -[a| ι]ₙ-> (ether, ι : p' |||| Π)
+
+(** spawning processes *)
+| n_spawn Π p p' v1 v2 l ι ι' ether:
+  mk_list v2 = Some l -> (ι : p |||| Π) ι' = None ->
+  p -⌈ASpawn ι' v1 v2⌉-> p'
+->
+  (ether, ι : p |||| Π) -[ASpawn ι' v1 v2 | ι]ₙ-> (ether, ι' : inl ([], EApp v1 l, [], [], false) |||| ι : p' |||| Π)
+
+(** Process termination, no more notifyable links *)
+| n_terminate ether ι Π :
+  (ether, ι : inr [] |||| Π) -[ATerminate | ι]ₙ-> (ether, Π -- ι)
+
+where "n -[ a | ι ]ₙ-> n'" := (nodeSemantics n a ι n').
+
+(** Refexive, transitive closure, with action logs: *)
+Reserved Notation "n -[ l ]ₙ->* n'" (at level 50).
+Inductive closureNodeSem : Node -> list (Action * PID) -> Node -> Prop :=
+| n_refl n (* n'  *): (* Permutation n n' -> *) n -[ [] ]ₙ->* n (* ' *)
+| n_trans n n' n'' l a ι:
+  n -[a|ι]ₙ-> n' -> n' -[l]ₙ->* n''
+->
+  n -[(a,ι)::l]ₙ->* n''
+where "n -[ l ]ₙ->* n'" := (closureNodeSem n l n').
+
+Theorem closureNodeSem_trans :
+  forall n n' l, n -[l]ₙ->* n' -> forall n'' l', n' -[l']ₙ->* n''
+->
+  n -[l ++ l']ₙ->* n''.
+Proof.
+  intros n n' l D1. induction D1; intros; simpl.
+  * exact H.
+  * eapply n_trans. exact H.
+    eapply IHD1 in H0. exact H0.
+Qed.
