src/Concurrent/ProcessSemantics.v
@@ -1,0 +1,348 @@
+(* This part of the work is based on https://dl.acm.org/doi/10.1145/3123569.3123576 *)
+From CoreErlang.FrameStack Require Export SubstSemantics.
+Require Export Coq.Sorting.Permutation.
+Require Export Coq.Classes.EquivDec.
+
+Import ListNotations.
+
+(* mailbox: [old msg₁, old msg₁, ...] ++ 
+            current msg₁ :: [new msg₁, new msg₂, ...] *)
+Definition Mailbox : Set := list Val * list Val.
+Definition ProcessFlag : Set := bool.
+Definition LiveProcess : Set := FrameStack * Redex * Mailbox * (list PID) * ProcessFlag.
+Definition DeadProcess : Set := list (PID * Val).
+Definition Process : Set := LiveProcess + DeadProcess.
+
+Inductive Signal : Set :=
+| Message (e : Val)
+| Exit (r : Val) (b : bool)
+| Link
+| Unlink.
+
+Inductive Action : Set :=
+| ASend (sender receiver : PID) (t : Signal)
+| AReceive (t : Exp)
+| AArrive (sender receiver : PID) (t : Signal)
+| ASelf (ι : PID)
+| ASpawn (ι : PID) (t1 t2 : Val)
+| τ
+| ATerminate
+| ASetFlag.
+
+Notation "x '.1'" := (fst x) (at level 20, left associativity).
+Notation "x '.2'" := (snd x) (at level 20, left associativity).
+
+Definition removeMessage (m : Mailbox) : option Mailbox :=
+  match m with
+  | (m1, msg :: m2) => Some (m1 ++ m2, [])
+  | _ => None
+  end.
+
+(* in Core Erlang, this function returns a flag and a message, if there is
+   a current message *)
+Definition peekMessage (m : Mailbox) : option Val :=
+  match m with
+  | (m1, msg :: m2) => Some msg
+  | _ => None
+  end.
+
+(* TODO: Check C implementation, how this exactly works *)
+Definition recvNext (m : Mailbox) : Mailbox :=
+  match m with
+  | (m1, msg :: m2) => (m1 ++ [msg], m2)
+  | (m1, [])        => (m1         , [])
+  end.
+
+Definition mailboxPush (m : Mailbox) (msg : Val) : Mailbox :=
+  (m.1, m.2 ++ [msg]).
+
+(* Since OTP 24.0, receive-s are syntactic sugars *)
+Definition EReceive l e :=
+  ELetRec [(0, 
+     °ELet 2 (EPrimOp "recv_peek_message" [])
+       (ECase (`VFunId (0, 0)) [
+         ([PLit (Atom "true")], `ttrue, °ECase (`VVar 1) (l ++
+           [([PVar], `ttrue, °ESeq (EPrimOp "recv_next" [])
+                                 (EApp (`VFunId (3, 0)) [])
+           )]));
+         ([PLit (Atom "false")], `ttrue,
+           °ELet 1 (EPrimOp "recv_wait_timeout" [])
+              (ECase (`VVar 0)
+                [([PLit (Atom "true")], `ttrue, e); (* TODO: timeout *)
+                 ([PLit (Atom "false")], `ttrue, °EApp (`VFunId (3, 0)) [])
+                ]
+              )
+         )
+       ])
+    )]
+    (EApp (`VFunId (0, 0)) []).
+
+(* Fixpoint find_clause (vs : list Val) (c : list (list Pat * Exp * Exp)) :
+  option (Exp * Exp) :=
+match c with
+| [] => None
+| (ps, g, e)::xs => match match_pattern_list ps vs with
+                     | None => find_clause vs xs
+                     | Some l => Some (g.[list_subst l idsubst],
+                                       e.[list_subst l idsubst])
+                    end
+end.
+
+Fixpoint receive (m : Mailbox) (c : list (list Pat * Exp * Exp)) : option (Exp * Exp) :=
+match m with
+| [] => None
+| m::ms => match find_clause [m] c with (* NOTE: this is the point where
+                                                 it is required that there
+                                                 is only one pattern in the
+                                                 clauses of receive *)
+           | Some res => Some res
+           | None => receive ms c
+           end
+end. *)
+
+(*
+  if a `receive` is evaluated:
+  1) try the first message against the clauses
+    a) if it matches one, evaluate its guard
+    b) if the guard is true, go to step 2)
+    c) if the guard is false, or the message did not match, save the message
+       into a separate cell, then evaluate `receive` with step 1), second message
+  2) remove the current message from the mailbox, re-build the mailbox with
+     the first part retrieved from the separate cell, and the second is the
+     current mailbox
+*)
+
+(* Definition pop (v : Val) (m : Mailbox) := removeFirst Exp_eq_dec v m.
+Definition etherPop := removeFirst (prod_eqdec Nat.eq_dec Exp_eq_dec). *)
+
+(* TODO: move this to Auxiliaries.v, and refactor eval_length *)
+Fixpoint len (l : Val) : option nat :=
+match l with
+| VNil => Some 0
+| VCons v1 v2 => match len v2 with
+                 | Some n2 => Some (S n2)
+                 | _ => None
+                 end
+| _ => None
+end.
+
+(* TODO: move this to Auxiliaries.v, and refactor eval_list_tuple *)
+Fixpoint mk_list (l : Val) : option (list Val) :=
+match l with
+| VNil => Some []
+| VCons v1 v2 => match mk_list v2 with
+                 | Some l => Some (v1 :: l)
+                 | _ => None
+                 end
+| _ => None
+end.
+
+Definition lit_from_bool (b : bool) : Val :=
+match b with
+| true => VLit "true"%string
+| false => VLit "false"%string
+end.
+Definition bool_from_lit (e : Val) : option bool :=
+match e with
+| VLit (Atom x) =>
+  if eqb x "true"%string
+  then Some true
+  else if eqb x "false"%string
+       then Some false
+       else None
+| _ => None
+end.
+
+(* Reserved Notation "p -⌈ a ⌉-> p'" (at level 50).
+Inductive processLocalSemantics : Process -> Action -> Process -> Prop :=
+
+(* correct evaluations *)
+| p_local fs e fs' e' mb :
+  ⟨fs, e⟩ --> ⟨fs', e'⟩
+->
+  (fs, e, mb) -⌈ τ ⌉-> (fs', e', mb)
+
+| p_arrive mb fs e v :
+  (fs, e, mb) -⌈ AArrive v ⌉-> (fs, e, mailboxPush mb v)
+
+| p_send ι mb fs v :
+  (FParams (ICall erlang send) [VPid ι] [] :: fs, RValSeq [v], mb)
+    -⌈ ASend ι v ⌉-> (fs, RValSeq [v], mb)
+
+| p_self ι mb fs :
+  (FParams (ICall erlang self) [] [] :: fs, RBox, mb)
+    -⌈ ASelf ι ⌉-> (fs, RValSeq [VPid ι], mb)
+
+| p_spawn ι mb fs l ext vars id e:
+  len l = Some vars ->
+  (FParams (ICall erlang spawn) [VClos ext id vars e] [] :: fs, RValSeq [l], mb)
+    -⌈ ASpawn ι (VClos ext id vars e) l ⌉-> (fs, RValSeq [VPid ι], mb)
+
+| p_recv_peek_message fs mb msg :
+  peekMessage mb = Some msg ->
+  (FParams (IPrimOp "recv_peek_message") [] [] :: fs, RBox, mb) -⌈τ⌉->
+    (fs, RValSeq [msg], mb)
+
+| p_recv_next fs mb :
+  (FParams (IPrimOp "recv_next") [] [] :: fs, RBox, mb) -⌈τ⌉->
+    (fs, RValSeq [ok], recvNext mb) (* TODO: in Core Erlang, this result cannot be observed *)
+
+| p_remove_message fs mb mb' :
+  removeMessage mb = Some mb' ->
+  (FParams (IPrimOp "remove_message") [] [] :: fs, RBox, mb) -⌈τ⌉->
+    (fs, RValSeq [ok], mb') (* TODO: in Core Erlang, this result cannot be observed *)
+
+(* exceptions *)
+| p_local_exc :
+  (FParams ident vl [], r, mb) -⌈τ⌉-> () 
+
+
+(*
+| p_receive mb l fs e m mb' bindings :
+  receive mb l = Some (m, e, bindings) -> mb' = pop m mb
+->
+  (fs, EReceive l, mb) -⌈ AReceive m ⌉-> (fs, e.[list_subst bindings idsubst], mb') *)
+
+where "p -⌈ a ⌉-> p'" := (processLocalSemantics p a p'). *)
+
+Reserved Notation "p -⌈ a ⌉-> p'" (at level 50).
+(*
+  Fredlund: https://www.diva-portal.org/smash/get/diva2:8988/FULLTEXT01.pdf
+  - it is similar, kill rules on page 66 are quite similar to our exit rules, and both differ from doc.
+*)
+Inductive processLocalSemantics : Process -> Action -> Process -> Prop :=
+(********** LOCAL STEPS **********)
+| p_local fs e fs' e' mb links flag :
+  ⟨fs, e⟩ --> ⟨fs', e'⟩
+->
+  inl (fs, e, mb, links, flag) -⌈ τ ⌉-> inl (fs', e', mb, links, flag)
+
+
+(********** SIGNAL ARRIVAL **********)
+(* message arrival *)
+| p_arrive mb fs e v flag links source dest :
+  inl (fs, e, mb, links, flag) -⌈ AArrive source dest (Message v) ⌉-> inl (fs, e, mailboxPush mb v, links, flag)
+
+(* exiting actions should come here *)
+(* dropping exit signals *)
+| p_exit_drop fs e mb links flag dest source reason b :
+  (
+    reason = normal /\ dest <> source /\ flag = false \/
+    ~ In source links /\ b = true /\ dest <> source
+                                           (*    ^------------ TODO: this check is missing from doc? *)
+  ) ->
+  inl (fs, e, mb, links, flag) -⌈ AArrive source dest (Exit reason b) ⌉->
+  inl (fs, e, mb, links, flag)
+(* terminating process *)
+| p_exit_terminate fs e mb links flag dest source reason reason' b :
+  (reason = kill /\ b = false /\ reason' = killed) \/
+  (flag = false /\ reason <> normal /\ reason' = reason /\ (b = true -> In source links) /\ 
+  (b = false -> reason <> kill))
+                  (*    ^------------ TODO: this check is missing from doc. *)
+ \/
+  (flag = false /\ reason = normal /\ source = dest /\ reason' = reason) ->
+  (*    ^------------ TODO: this check is missing from doc. *)
+  inl (fs, e, mb, links, flag) -⌈ AArrive source dest (Exit reason b) ⌉->
+  inr (map (fun l => (l, reason')) links)
+(* convert exit signal to message *)
+(* TODO, NOTE: here tuple should be used instead of list! *)
+| p_exit_convert fs e mb links dest source reason b:
+  (b = false /\ reason <> kill) \/
+  (b = true /\ In source links)
+ ->
+  inl (fs, e, mb, links, true) -⌈ AArrive source dest (Exit reason b) ⌉->
+  inl (fs, e, mailboxPush mb (VCons EXIT 
+                           (VCons (VPid source) (VCons reason VNil))), links, true)
+(* link received *)
+| p_link_arrived fs e mb links source dest flag:
+  inl (fs, e, mb, links, flag) -⌈AArrive source dest Link⌉->
+  inl (fs, e, mb, source :: links, flag)
+
+(* unlink received *)
+| p_unlink_arrived fs e mb links source dest flag :
+  inl (fs, e, mb, links, flag) -⌈AArrive source dest Unlink⌉->
+  inl (fs, e, mb, remove Nat.eq_dec source links, flag)
+
+(********** SIGNAL SENDING **********)
+(* message send *)
+| p_send ι v mb fs flag links source :
+  inl (FParams (ICall erlang send) [VPid ι] [] :: fs, RValSeq [v], mb, links, flag)
+  -⌈ ASend source ι (Message v) ⌉-> inl (fs, RValSeq [v], mb, links, flag)
+(* exit, 2 parameters *)
+| p_exit fs v mb flag ι selfι links :
+  inl (FParams (ICall erlang exit) [VPid ι] [] :: fs, RValSeq [v], mb, links, flag) -⌈ ASend selfι ι (Exit v false) ⌉->
+  inl (fs, RValSeq [ttrue], mb, links, flag)
+(* link *)
+| p_link fs ι mb flag links selfι :
+  inl (FParams (ICall erlang link) [] [] :: fs, RValSeq [VPid ι], mb, links, flag)
+  -⌈ASend selfι ι Link⌉->
+  inl (fs, RValSeq [ok], mb, ι :: links, flag)
+(* unlink *)
+| p_unlink fs ι mb flag links selfι :
+  inl (FParams (ICall erlang unlink) [] [] :: fs, RValSeq [VPid ι], mb, links, flag) 
+  -⌈ASend selfι ι Unlink⌉->
+  inl (fs, RValSeq [ok], mb, remove Nat.eq_dec ι links, flag)
+(* DEAD PROCESSES *)
+| p_dead ι selfι links reason:
+  inr ((ι, reason) :: links) -⌈ASend selfι ι (Exit reason true)⌉-> inr links
+
+
+(********** SELF **********)
+(* self *)
+| p_self ι fs mb flag links :
+  inl (FParams (ICall erlang self) [] [] :: fs, RBox, mb, links, flag) -⌈ ASelf ι ⌉-> inl (fs, RValSeq [VPid ι], mb, links, flag)
+
+(********** SPAWN **********)
+(* spawn *)
+| p_spawn ι fs mb ext id vars e l flag links :
+  Some vars = len l ->
+  inl (FParams (ICall erlang spawn) [VClos ext id vars e] [] :: fs, RValSeq [l], mb, links, flag)
+    -⌈ASpawn ι (VClos ext id vars e) l⌉-> inl (fs, RValSeq [VPid ι], mb, links, flag)
+
+(********** RECEVIE **********)
+| p_recv_peek_message fs mb msg links flag :
+  peekMessage mb = Some msg ->
+  inl (FParams (IPrimOp "recv_peek_message") [] [] :: fs, RBox, mb, links, flag) -⌈τ⌉->
+    inl (fs, RValSeq [msg], mb, links, flag)
+
+| p_recv_next fs mb links flag:
+  inl (FParams (IPrimOp "recv_next") [] [] :: fs, RBox, mb, links, flag) -⌈τ⌉->
+    inl (fs, RValSeq [ok], recvNext mb, links, flag) (* TODO: in Core Erlang, this result cannot be observed *)
+
+| p_remove_message fs mb mb' links flag:
+  removeMessage mb = Some mb' ->
+  inl (FParams (IPrimOp "remove_message") [] [] :: fs, RBox, mb, links, flag) -⌈τ⌉->
+    inl (fs, RValSeq [ok], mb', links, flag) (* TODO: in Core Erlang, this result cannot be observed *)
+
+(********** PROCESS FLAG **********)
+(* Replace process flags *)
+| p_set_flag fs mb flag y v links :
+  Some y = bool_from_lit v ->
+  inl (FParams (ICall erlang self) [] [] :: fs, RValSeq [v], mb, links, flag) 
+   -⌈ ASetFlag ⌉-> inl (fs, RValSeq [lit_from_bool flag], mb, links, y)
+
+(********** TERMINATION **********)
+(* termination *)
+| p_terminate v mb links flag:
+  (* NOTE: "singletonness" is checked in compile time in Core Erlang *)
+  inl ([], RValSeq [v], mb, links, flag) -⌈ATerminate⌉->
+   inr (map (fun l => (l, normal)) links) (* NOTE: is internal enough here? - no, it's not for bisimulations *)
+
+(* exit with one parameter <- this is sequential, it's in FrameStack/Auxiliaries.v *)
+
+(********** EXCEPTIONS **********)
+(* creation *)
+| p_terminate_exc exc mb links flag:
+  (* NOTE: if the final result is an exception, it's reason is sent
+     to the linked processes *)
+  inl ([], RExc exc, mb, links, flag) -⌈ATerminate⌉->
+   inr (map (fun l => (l, exc.1.2)) links)
+
+where "p -⌈ a ⌉-> p'" := (processLocalSemantics p a p').
+
+Inductive LabelStar {A B : Type} (r : A -> B -> A -> Prop) : A -> list B -> A -> Prop :=
+| lsrefl x : LabelStar r x [] x
+| lsstep x l ls y z : r x l y -> LabelStar r y ls z -> LabelStar r x (l::ls) z.
+
+Notation "x -⌈ xs ⌉->* y" := (LabelStar processLocalSemantics x xs y) (at level 50).
+
